some lemmas

src/assoc.v
@@ -1,16 +1,18 @@
 (* From mathcomp Require Import ssreflect.seq all_ssreflect. *)
 From Paco Require Import paco pacotac.
 From SST Require Import src.expr src.header src.local CpdtTactics src.lcontext.
-From SST Require Import src.global src.projection src.part src.balanced.
-From SST Require Import lemma.projection lemma.projection_helper.
+From SST Require Import src.global src.projection src.part  src.balanced src.merge src.gttreeh.
+From SST Require Import lemma.projection lemma.projection_helper lemma.decidable.
 Require Import List String Coq.Arith.PeanoNat Morphisms Relations Setoid.
 Require Import Coq.Program.Equality.
 Import ListNotations.
 
 
-Definition issubProj (t:ltt) (g:gtt) (p:part) := exists tg, projectionC g p tg /\ subtypeC t tg.
+Definition issubProj (t:ltt) (g:gtt) (p:part) := 
+    exists tg, projectionC g p tg /\ subtypeC t tg.
 
 Search subtypeC.
+
 
 Definition assoc (g: tctx) (gt:gtt) := 
     forall p, (isgPartsC p gt -> exists Tp, M.find p g=Some Tp /\  
@@ -18,7 +20,7 @@ Definition assoc (g: tctx) (gt:gtt) :=
          ~ isgPartsC p gt -> forall Tpx, M.find p g = Some Tpx -> Tpx=ltt_end.
 
 Definition send_cond (xs:list (option (sort*ltt))) (ys:list (option (sort*gtt))) (p:part) := 
-    Forall2 (fun x y => x=None 
+    Forall2R (fun x y => x=None 
         \/ (exists s elx s' ely, y=Some (s',ely)/\ x=Some (s,elx) /\ 
         subsort s s' /\
         issubProj elx ely p)) xs ys.
@@ -35,9 +37,191 @@ Definition send_cond2 (t:ltt) (ys:list(option(sort*gtt))) (p:part) :=
     Forall (fun y=> (y=None)\/ 
     (exists s' Gy, y=Some (s', Gy) /\issubProj t Gy p)) ys.
 
-Locate proj_inv_lis.
+Lemma subtype_send_inv1 : forall q xs T, 
+subtypeC (ltt_send q xs) T -> exists ys, T=ltt_send q ys.
+Proof.
+    intros.
+    destruct T eqn:Ht;first (apply subtype_end_inv in H; crush);
+    destruct (Nat.eq_dec n q);try (exists l);crush;
+    pinversion H;crush;apply subtype_monotone.
+Qed. 
+Print gtth.
+(*
+Definition option_max x y :=
+    match (x,y) with 
+        | (None, None) => None
+        | (Some a, Some b) => Some (max a b)
+        | (Some a, None) => Some a
+        | (None, Some b) => Some b
+    end. 
+Fixpoint extract_hs (hs:list (option (sort * gtth))) := 
+    match hs with 
+        | [] => []
+        | None::ys => None::extract_hs ys
+        | Some (s,a)::ys => Some a :: extract_hs ys end.
+Fixpoint context_height (h:gtth) :=
+    match h with 
+        | gtth_hol n => Some 0
+        | gtth_send p q hs => seq.foldr option_max None (extract_hs hs)
+    end.  *)
+(* context_height h x means height of h <= x*)
+Inductive context_height: gtth -> nat -> Prop :=
+    | height_hole: forall n x, context_height (gtth_hol n) x
+    | height_send: forall p q hs x, 
+        SList hs -> Forall (fun u=> u=None \/ 
+            (exists s h, u=Some (s,h) /\ context_height h x)) hs->
+        context_height (gtth_send p q hs) (S x).
+        
+Section height_induction.
+    
+End height_induction.
 
-Lemma subproj_inv_send: forall q xs p G, wfgC G -> issubProj (ltt_send q xs) G p -> 
+Lemma subtype_recv_inv1 : forall q xs T, 
+subtypeC (ltt_recv q xs) T -> exists ys, T=ltt_recv q ys.
+Proof.
+    intros.
+    destruct T eqn:Ht;first (apply subtype_end_inv in H; crush);
+    destruct (Nat.eq_dec n q);try (exists l);crush;
+    pinversion H;crush;apply subtype_monotone.
+Qed.
+
+Lemma subtype_send_strong_inv: forall pt xs T, 
+subtypeC (ltt_send pt xs) T -> 
+exists ys, T=ltt_send pt ys /\
+Forall2R
+(fun u v : option (sort * ltt) =>
+u = None \/
+(exists (s s' : sort) (t t' : ltt),
+u = Some (s, t) /\
+v = Some (s', t') /\ subsort s s' /\ subtypeC t t'))
+xs ys.
+Proof.
+    intros.
+    pose proof H as H'.
+    apply subtype_send_inv1 in H. destr_hyps. subst.
+    apply subtype_send_inv in H'. exists x. easy.
+Qed.
+
+Lemma subtype_recv_strong_inv: forall pt xs T, 
+subtypeC (ltt_recv pt xs) T -> 
+exists ys, T=ltt_recv pt ys /\
+Forall2R
+(fun u v : option (sort * ltt) =>
+u = None \/
+(exists (s s' : sort) (t t' : ltt),
+u = Some (s, t) /\
+v = Some (s', t') /\ subsort s s' /\
+subtypeC t' t)) ys xs.
+Proof.
+    intros.
+    pose proof H as H'.
+    apply subtype_recv_inv1 in H. destr_hyps. subst.
+    apply subtype_recv_inv in H'. exists x. easy.
+Qed.
+Search wfG.
+Lemma empty_not_wfg : forall p q, ~ wfgC (gtt_send p q []).
+Proof.
+    unfold not;intros. unfold wfgC in H. destr_hyps.
+    induction x;(try (pinversion H;apply gttT_mon)).
+    pinversion H;subst. destruct l.
+    inversion H0;subst. inversion H7.
+    inversion H4. apply gttT_mon.
+
+Admitted.
+Ltac invalid_forall_wfg :=
+    try ((match goal with | 
+    [H:Forall2 _  (?a::?b) [] |- _] => inversion H 
+    | [H:Forall2 _  [] (?a::?b)  |- _] => inversion H 
+    | [H:Forall2R _ (?a::?b) [] |- _] => inversion H
+    | [H:wfgC (gtt_send _ _ []) |- _] => apply empty_not_wfg in H end);
+    contradiction).
+
+Lemma onth_exists {A:Type}: forall n (xs: list (option A)) a p, 
+onth n xs = Some a -> ~ p (Some a) -> ~ Forall p xs.
+Proof.
+    unfold not.
+    intros.
+    generalize dependent n. 
+    generalize dependent xs.
+    induction xs;intros;[| inversion H1; subst; specialize (IHxs H5)];
+    destruct n; crush.
+Qed.
+
+Lemma onth_nil {A:Type}: forall n, onth  n ([]:list (option A))= None.
+Proof. intros;destruct n;unfold onth in *;crush. Qed.
+
+Lemma projection_implies_part :forall g p q xs, 
+projectionC g p (ltt_send q xs) -> isgPartsC p g.
+Proof.
+    intros. pinversion H;subst;crush. apply proj_mon.
+Qed.
+Lemma empty_not_wfg_proj: forall p q g, wfgC g -> projectionC g p (ltt_send q []) -> False.
+Proof. 
+Admitted.
+Lemma subproj_helper: forall xs ys gs p,  Forall2R
+(fun u v : option (sort * ltt) =>
+u = None \/
+(exists (s s' : sort) (t t' : ltt),
+u = Some (s, t) /\
+v = Some (s', t') /\ subsort s s' /\ subtypeC t t'))
+xs ys -> Forall2
+(fun (u : option (sort * gtt)) (v : option (sort * ltt)) =>
+u = None /\ v = None \/
+(exists (s : sort) (g : gtt) (t : ltt),
+u = Some (s, g) /\
+v = Some (s, t) /\ upaco3 projection bot3 g p t))
+gs ys -> Forall2R
+(fun (x : option (sort * ltt)) (y : option (sort * gtt)) =>
+x = None \/
+(exists (s : sort) (elx : ltt) (s' : sort) (ely : gtt),
+y = Some (s', ely) /\
+x = Some (s, elx) /\ subsort s s' /\ issubProj elx ely p)) xs gs.
+Proof.
+    intros xs.
+    induction xs; intros; destruct ys;
+    destruct gs;try invalid_forall_wfg;crush. constructor. constructor.
+    constructor.
+    destruct a;crush. right. inversion H. inversion H0. destruct H4;destruct H10;crush.
+    exists x2, x4, x3,x0. unfold issubProj. crush. exists x5. destruct H5;crush.
+    inversion H;inversion H0;subst. eapply IHxs with (gs:=gs) (ys:=ys);crush.
+Qed.
+Check M.merge.
+
+Lemma subproj_inv_send: forall q xs p G, wfgC G -> 
+    SList xs -> issubProj (ltt_send q xs) G p -> 
     (exists ys, G=gtt_send p q ys /\ send_cond xs ys p)
     \/ (exists s t ys, G=gtt_send s t ys /\ p <> s /\ p<> t /\ 
         send_cond2 (ltt_send q xs) ys p ).
+Proof.
+    intros.
+    unfold issubProj in H1.
+    destr_hyps.
+    
+    apply subtype_send_strong_inv in H2.
+    destruct H2. destruct H2. subst.
+    rename H3 into Hsubtpcond.
+    (*ltt_send q x0 is the supertype*)
+    Print projection.
+    pinversion H1; try apply proj_mon; subst.
+    {
+        
+        (*G=gtt_send r q xs0*)
+        rename H8 into Hprojcond.
+        left. exists xs0. split; try reflexivity. subst.
+        unfold send_cond.
+        destruct xs; destruct xs0;crush;destruct x0;
+        try (match goal with | 
+            [H:Forall2 _  (?a::?b) [] |- _] => inversion H 
+            | [H:Forall2 _  [] (?a::?b)  |- _] => inversion H 
+            | [H:wfgC (gtt_send _ _ []) |- _] => apply empty_not_wfg in H end);
+        crush.
+        eapply subproj_helper with(ys:=o1::x0);crush.
+    }
+    {
+
+        right. exists p0,q0,xs0. unfold send_cond2. crush. 
+        unfold issubProj.
+        (*ys: list that merges to ltt_send q x0*)
+        inversion H1;subst. crush.
+    }
+Qed.
